finish stepping through key expansion (modulo some admits)
proof is too big to Qed, will have to split

aes/verif_setkey_enc_LL.v
@@ -87,7 +87,11 @@ Fixpoint pow_fun{T: Type}(f: T -> T)(n: nat)(a: T): T := match n with
 | S m => f (pow_fun f m a)
 end.
 
-Definition KeyExpansion: list int -> list int := pow_fun GrowKeyByOne (Z.to_nat (Nb*(Nr+1))).
+(* +2 because 1 is for the initial round which is not counted, and 1 superfluous round key is
+   created in the last loop iteration, because each iteration creates 2 round keys.
+   -Nk because the first two round keys are just the unexpanded key.
+  Note that (Nb*(Nr+2)-Nk) = 56. *)
+Definition KeyExpansion: list int -> list int := pow_fun GrowKeyByOne (Z.to_nat (Nb*(Nr+2)-Nk)).
 
 (* arr: list of bytes *)
 Definition get_uint32_le (arr: list Z) (i: Z) : int :=
@@ -97,16 +101,31 @@ Definition get_uint32_le (arr: list Z) (i: Z) : int :=
    (Int.shl (Int.repr (Znth (i+2) arr 0)) (Int.repr 16)))
    (Int.shl (Int.repr (Znth (i+3) arr 0)) (Int.repr 24))).
 
-Definition key_bytes_to_key_words(key_bytes: list Z): list int := [
-  get_uint32_le key_bytes 0;
-  get_uint32_le key_bytes 4;
-  get_uint32_le key_bytes 8;
-  get_uint32_le key_bytes 12;
-  get_uint32_le key_bytes 16;
-  get_uint32_le key_bytes 20;
-  get_uint32_le key_bytes 24;
-  get_uint32_le key_bytes 28
-].
+Definition partially_filled(i n: Z)(f: Z -> int): list val := 
+  (map Vint (fill_list i f)) ++ (repeat_op_table (n-i) Vundef id).
+
+Lemma update_partially_filled: forall (i: Z) (n: Z) (f: Z -> int),
+  0 <= i < n ->
+  upd_Znth i (partially_filled i n f) (Vint (f i))
+  = partially_filled (i+1) n f.
+Admitted.
+
+Lemma Znth_partially_filled: forall (i j n: Z) (f: Z -> int),
+  0 <= i -> i < j -> j <= n ->
+  Znth i (partially_filled j n f) Vundef = Vint (f i).
+Admitted.
+
+Definition key_bytes_to_key_words(key_bytes: list Z): list int := 
+  fill_list 8 (fun i => get_uint32_le key_bytes (i*4)).
+
+(*
+Definition append_4_bytes_as_word(bytes: list Z)(words: list int): list int :=
+  let i := Zlength words in
+  words ++ [get_uint32_le bytes (i*4)].
+
+Definition key_bytes_to_key_words(key_bytes: list Z): list int := 
+  pow_fun (append_4_bytes_as_word key_bytes) 8%nat [].
+*)
 
 (* Note: clightgen turns global variables of type int to pointers to int, to make them addressable,
    so aes_init_done is a pointer to int, not an int! *)
@@ -121,19 +140,23 @@ Definition key_expansion_spec :=
       LOCAL (temp _ctx ctx; temp _key key; temp _keybits (Vint (Int.repr 256)); 
              gvar _aes_init_done aes_init_done;
              gvar _tables tables)
-      SEP (data_at_ ctx_sh t_struct_aesctx ctx;
+      SEP (data_at ctx_sh t_struct_aesctx 
+                   (Vint Int.zero,
+                   (nullval, 
+                   (map Vint (repeat_op_table 68 Int.zero id)))) ctx;
            data_at key_sh (tarray tuchar (4*8)) (map Vint (map Int.repr key_chars)) key;
            (*if init_done ?= 1 then tables_initialized tables else tables_uninitialized tables*)
            data_at ish tint (Vint (Int.repr init_done)) aes_init_done;
            tables_initialized tables)
     POST [  tint ]
       PROP () 
-      LOCAL (temp ret_temp (Vint Int.zero); gvar _aes_init_done aes_init_done)
+      LOCAL (temp ret_temp (Vint Int.zero))
       SEP (data_at key_sh (tarray tuchar (4*8)) (map Vint (map Int.repr key_chars)) key;
            data_at ctx_sh t_struct_aesctx 
-                   (Vint (Int.repr 8),
-                   (Vint (Int.repr (nested_field_offset t_struct_aesctx [StructField _buf])), 
-                   (map Vint [] (*TODO*)))) ctx;
+                   (Vint (Int.repr 14),
+                   ((field_address t_struct_aesctx [StructField _buf] ctx), 
+                   (map Vint (KeyExpansion (key_bytes_to_key_words key_chars))
+                    ++ (repeat_op_table 4 (Vint Int.zero) id)))) ctx;
            data_at ish tint (Vint (Int.repr init_done)) aes_init_done;
            tables_initialized tables).
 
@@ -175,13 +198,53 @@ Definition first_loop_inv00 ctx key tables aes_init_done init_done key_chars ctx
       field_at ctx_sh t_struct_aesctx [StructField _rk] 
         (field_address t_struct_aesctx [StructField _buf] ctx) ctx;
       field_at ctx_sh t_struct_aesctx [StructField _buf]
-        (map Vint (map Int.repr (sublist 0 i key_chars)) ++ (repeat Vundef (Z.to_nat (68-i)))) ctx;
+        (partially_filled i 68 (fun i => get_uint32_le key_chars (i*4))) ctx;
       data_at key_sh (tarray tuchar (4 * 8)) (map Vint (map Int.repr key_chars)) key;
       data_at ish tint (Vint (Int.repr init_done)) aes_init_done;
       tables_initialized tables).
 
 Definition first_loop_inv0 ctx key tables aes_init_done init_done key_chars ctx_sh key_sh ish :=
   EX i: Z, first_loop_inv00 ctx key tables aes_init_done init_done key_chars ctx_sh key_sh ish i.
+
+Definition main_loop_invariant0 ctx key tables ctx_sh key_sh ish key_chars aes_init_done init_done i :=
+  PROP ( )
+  LOCAL (
+    temp _RK (offset_val (i*32) (field_address t_struct_aesctx [StructField _buf] ctx));
+    temp _ctx ctx;
+    gvar _tables tables
+  ) SEP (
+    field_at ctx_sh t_struct_aesctx [StructField _nr] (Vint (Int.repr 14)) ctx;
+    field_at ctx_sh t_struct_aesctx [StructField _rk]
+      (field_address t_struct_aesctx [StructField _buf] ctx) ctx;
+    field_at ctx_sh t_struct_aesctx [StructField _buf]
+      (map Vint (pow_fun GrowKeyByOne (Z.to_nat (i*8)) (key_bytes_to_key_words key_chars))
+      ++ repeat_op_table (60-i*8) Vundef id) ctx;
+    data_at key_sh (tarray tuchar (4 * 8)) (map Vint (map Int.repr key_chars)) key;
+    data_at ish tint (Vint (Int.repr init_done)) aes_init_done;
+    tables_initialized tables
+  ).
+
+Definition main_loop_invariant ctx key tables ctx_sh key_sh ish key_chars aes_init_done init_done :=
+  EX i: Z, main_loop_invariant0 ctx key tables ctx_sh key_sh ish key_chars aes_init_done init_done i.
+
+Lemma Znth_partially_expanded_key: forall i j key,
+  0 <= i < 7 ->
+  0 <= j < 8 + i*8 ->
+  (Znth j (map Vint (pow_fun GrowKeyByOne (Z.to_nat (i * 8)) key)
+           ++ repeat_op_table (60 - i * 8) Vundef id) Vundef)
+  = Vint (Znth j (KeyExpansion key) Int.zero).
+Admitted.
+
+Lemma Zlength_partially_expanded_key: forall i key_chars,
+  0 <= i < 7 ->
+  Zlength key_chars = 32 ->
+  Zlength (map Vint (pow_fun GrowKeyByOne (Z.to_nat (i * 8)) (key_bytes_to_key_words key_chars)) ++
+          repeat_op_table (60 - i * 8) Vundef id) = 68.
+Admitted.
+
+Lemma masked_byte_range: forall i,
+  0 <= Z.land i 255 < 256.
+Admitted.
 
 Lemma body_key_expansion: semax_body Vprog Gprog f_mbedtls_aes_setkey_enc key_expansion_spec.
 Proof.
@@ -229,9 +292,149 @@ Proof.
       else Vundef) = field_address t_struct_aesctx [StructField _buf] ctx) by entailer!.
     forward.
     entailer!.
-    admit.
+    replace (4 * i)%Z with (i * 4)%Z by omega.
+    fold ((fun i0 => get_uint32_le key_chars (i0 * 4)) i).
+    rewrite update_partially_filled by omega.
+    apply derives_refl.
   }
   reassoc_seq.
   (* main loop: *)
 
-Qed.
+  (* TODO floyd: we can only use forward_for_simple_bound because we moved the "RK += 8" from the 
+     increment to the end of the loop body *)
+  forward_for_simple_bound 7
+    (main_loop_invariant ctx key tables ctx_sh key_sh ish key_chars aes_init_done init_done).
+  { (* precondition implies loop invariant: *)
+    (* TODO floyd: this should be automatic, and entailer should not clear the P I'm asserting here *)
+    assert_PROP (isptr (field_address t_struct_aesctx [StructField _buf] ctx)) as P by entailer!.
+    change (0 * 32)%Z with 0.
+    rewrite isptr_offset_val_zero by assumption.
+    entailer!. }
+  { (* loop body preserves invariant: *)
+    assert_PROP (forall j, 0 <= j < 16 -> force_val
+      (sem_add_pi tuint (offset_val (i * 32) (field_address t_struct_aesctx [StructField _buf] ctx))
+      (Vint (Int.repr j)))
+      = field_address t_struct_aesctx [ArraySubsc (i*8+j); StructField _buf] ctx) as E. {
+      assert_PROP (isptr ctx) as P by entailer!. destruct ctx; inv P.
+      entailer!.
+      intros j B.
+      rewrite field_compatible_field_address by assumption.
+      rewrite field_compatible_field_address by auto with field_compatible.
+      simpl. rewrite Int.add_assoc. rewrite add_repr. do 4 f_equal. omega.
+    }
+
+    (* TODO floyd: In these two tactics, entailer! does not solve everything, but entailer works *)
+
+    Ltac RK_load E j :=
+      let A := fresh "A" in let E2 := fresh "E" in
+      assert (0 <= j < 16) as A by omega;
+      pose proof (E _ A) as E2; clear A;
+      forward;
+      repeat rewrite upd_Znth_diff by (repeat rewrite upd_Znth_Zlength; omega);
+      repeat rewrite upd_Znth_same by (repeat rewrite upd_Znth_Zlength; omega);
+      rewrite ?Znth_partially_expanded_key by omega; [ entailer | ];
+      clear E2.
+
+    Ltac RK_store E j :=
+      let A := fresh "A" in let E2 := fresh "E" in
+      assert (0 <= j < 16) as A by omega;
+      pose proof (E _ A) as E2; clear A;
+      forward; [ entailer | ];
+      clear E2.
+
+    Arguments Z.land _ _ : simpl never.
+
+    pose proof (Zlength_partially_expanded_key i key_chars) as L.
+    spec L; [ omega | ]. spec L; [ assumption | ].
+
+    RK_load E 0.
+    RK_load E 7.
+    unfold tables_initialized.
+    Transparent RCON.
+    assert (Zlength RCON = 10) by reflexivity.
+    forward.
+    pose proof masked_byte_range.
+    forward. forward.
+    forward. forward.
+    fold (tables_initialized tables).
+    simpl.
+    RK_store E 8.
+    RK_load E 1.
+    RK_load E 8.
+    RK_store E 9.
+    RK_load E 2.
+    RK_load E 9.
+    RK_store E 10.
+    RK_load E 3.
+    RK_load E 10.
+    RK_store E 11.
+
+    RK_load E 4.
+    RK_load E 11.
+    unfold tables_initialized.
+    pose proof masked_byte_range.
+    forward. forward.
+    forward. forward.
+    fold (tables_initialized tables).
+    simpl.
+    RK_store E 12.
+    RK_load E 5.
+    RK_load E 12.
+    RK_store E 13.
+    RK_load E 6.
+    RK_load E 13.
+    RK_store E 14.
+    RK_load E 7.
+    RK_load E 14.
+    RK_store E 15.
+
+    forward. {
+      entailer.
+    }
+    assert_PROP (isptr ctx) as P by entailer!. destruct ctx; inv P.
+    entailer!.
+    - simpl. rewrite E by omega.
+      rewrite field_compatible_field_address by assumption.
+      rewrite field_compatible_field_address by auto with field_compatible.
+      simpl. rewrite Int.add_assoc. do 2 f_equal. rewrite add_repr. f_equal. omega.
+    - clear H10.
+
+Lemma update_partially_expanded_key: forall j v key_chars,
+(* TODO what's the value of v? *)
+  upd_Znth (j + 8) (map Vint (pow_fun GrowKeyByOne (Z.to_nat j) (key_bytes_to_key_words key_chars))
+                   ++ repeat_op_table (60 - j) Vundef id) v
+  = (map Vint (pow_fun GrowKeyByOne (Z.to_nat (j + 1)) (key_bytes_to_key_words key_chars))
+                   ++ repeat_op_table (60 - (j + 1)) Vundef id).
+Admitted.
+      rewrite update_partially_expanded_key.
+      replace (i * 8 + 9) with (i * 8 + 1 + 8) by omega.
+      rewrite update_partially_expanded_key.
+      replace (i * 8 + 10) with (i * 8 + 1 + 1 + 8) by omega.
+      rewrite update_partially_expanded_key.
+      replace (i * 8 + 11) with (i * 8 + 1 + 1 + 1 + 8) by omega.
+      rewrite update_partially_expanded_key.
+      replace (i * 8 + 12) with (i * 8 + 1 + 1 + 1 + 1 + 8) by omega.
+      rewrite update_partially_expanded_key.
+      replace (i * 8 + 13) with (i * 8 + 1 + 1 + 1 + 1 + 1 + 8) by omega.
+      rewrite update_partially_expanded_key.
+      replace (i * 8 + 14) with (i * 8 + 1 + 1 + 1 + 1 + 1 + 1 + 8) by omega.
+      rewrite update_partially_expanded_key.
+      replace (i * 8 + 15) with (i * 8 + 1 + 1 + 1 + 1 + 1 + 1 + 1 + 8) by omega.
+      rewrite update_partially_expanded_key.
+      replace (i * 8 + 1 + 1 + 1 + 1 + 1 + 1 + 1 + 1) with ((i + 1) * 8)%Z by omega.
+      apply derives_refl.
+  }
+  (* return 0 *)
+  assert ((Nb * (Nr + 2) - Nk) = 7 * 8)%Z as E by reflexivity.
+  rewrite <- E.
+  progress fold (KeyExpansion (key_bytes_to_key_words key_chars)).
+  rewrite E. clear E. change (60 - 7 * 8) with 4.
+  forget (KeyExpansion (key_bytes_to_key_words key_chars)) as R.
+  forward.
+(* TODO this does not hold, we have to replace Vundef by (Vint Int.zero) in the whole proof *)
+Lemma Vundef_is_Vint:
+  repeat_op_table 4 Vundef id = repeat_op_table 4 (Vint Int.zero) id.
+Admitted.
+  rewrite Vundef_is_Vint.
+  unfold_data_at 4%nat. entailer!.
+Time Qed. (* takes too long, using 25% CPU only *)
